add _TS version of repl_types and prove relation

compiler/repl/repl_typesScript.sml
@@ -69,12 +69,55 @@ Inductive repl_types:
      repl_types b (ffi,rs) (types,s with refs := new_store,env))
 End
 
-Definition ref_lookup_ok_def:
-  ref_lookup_ok refs (name:(string,string) id,ty,loc) =
-    ∃v:semanticPrimitives$v.
-      store_lookup loc refs = SOME (Refv v) ∧
-      (ty = Bool ⇒ v = Boolv T ∨ v = Boolv F) ∧
-      (ty = Str ⇒ ∃t. v = Litv (StrLit t))
+(* Mirror definitions for repl_types using the type system directly *)
+Definition to_type_TS_def:
+  to_type_TS Bool = Tapp [] Tbool_num ∧
+  to_type_TS Str  = Tapp [] Tstring_num ∧
+  to_type_TS Exn  = Tapp [] Texn_num
+End
+
+Definition check_ref_types_TS_def:
+  check_ref_types_TS types (env :semanticPrimitives$v sem_env) (name,ty,loc) ⇔
+    nsLookup types.v name = SOME (0,Tapp [to_type_TS ty] Tref_num) ∧
+    nsLookup env.v name = SOME (Loc loc)
+End
+
+Inductive repl_types_TS:
+[repl_types_TS_init:]
+  (∀ffi rs decs tids tenv (s:'ffi semanticPrimitives$state) env.
+     type_ds T prim_tenv decs tids tenv ∧
+     evaluate$evaluate_decs (init_state ffi) init_env decs = (s,Rval env) ∧
+     EVERY (check_ref_types_TS (extend_dec_tenv tenv prim_tenv) (extend_dec_env env init_env)) rs ⇒
+     repl_types_TS (ffi,rs) (extend_dec_tenv tenv prim_tenv,s,extend_dec_env env init_env)) ∧
+[repl_types_TS_eval:]
+  (∀ffi rs decs tenv (s:'ffi semanticPrimitives$state) env
+    new_tids new_tenv new_env new_s.
+     repl_types_TS (ffi,rs) (tenv,s,env) ∧
+     type_ds T tenv decs new_tids new_tenv ∧
+     evaluate$evaluate_decs s env decs = (new_s,Rval new_env) ⇒
+     repl_types_TS (ffi,rs) (extend_dec_tenv new_tenv tenv,new_s,extend_dec_env new_env env)) ∧
+[repl_types_TS_exn:]
+  (∀ffi rs decs tenv (s:'ffi semanticPrimitives$state) env
+    new_tids new_tenv new_s e.
+     repl_types_TS (ffi,rs) (tenv,s,env) ∧
+     type_ds T tenv decs new_tids new_tenv ∧
+     evaluate$evaluate_decs s env decs = (new_s,Rerr (Rraise e)) ⇒
+     repl_types_TS (ffi,rs) (tenv,new_s,env)) ∧
+[repl_types_TS_exn_assign:]
+  (∀ffi rs decs tenv (s:'ffi semanticPrimitives$state) env
+    new_tids new_tenv new_s e name loc new_store.
+     repl_types_TS (ffi,rs) (tenv,s,env) ∧
+     type_ds T tenv decs new_tids new_tenv ∧
+     evaluate$evaluate_decs s env decs = (new_s,Rerr (Rraise e)) ∧
+     MEM (name,Exn,loc) rs ∧
+     store_assign loc (Refv e) new_s.refs = SOME new_store ⇒
+     repl_types_TS (ffi,rs) (tenv,new_s with refs := new_store,env)) ∧
+[repl_types_TS_str_assign:]
+  (∀ffi rs tenv (s:'ffi semanticPrimitives$state) env t name loc new_store.
+     repl_types_TS (ffi,rs) (tenv,s,env) ∧
+     MEM (name,Str,loc) rs ∧
+     store_assign loc (Refv (Litv (StrLit t))) s.refs = SOME new_store ⇒
+     repl_types_TS (ffi,rs) (tenv,s with refs := new_store,env))
 End
 
 Theorem init_config_tenv_to_ienv:
@@ -82,6 +125,12 @@ Theorem init_config_tenv_to_ienv:
 Proof
   rw[init_config_def, tenv_to_ienv_def]
   \\ EVAL_TAC
+QED
+
+Theorem ienv_to_tenv_init_config:
+  ienv_to_tenv init_config = prim_tenv
+Proof
+  EVAL_TAC
 QED
 
 Theorem tenv_ok_prim_tenv[simp]:
@@ -112,6 +161,124 @@ Proof
   \\ rw[] \\ simp[]
   \\ EVAL_TAC \\ simp[]
 QED
+
+Theorem ienv_ok_init_config:
+  ienv_ok {} init_config
+Proof
+  EVAL_TAC>>
+  CONJ_TAC>- (
+    Induct>>
+    simp[namespaceTheory.nsLookup_def])>>
+  CONJ_TAC>- (
+    Induct>>
+    simp[namespaceTheory.nsLookup_def]>>
+    rw[]>>EVAL_TAC)>>
+  Induct>>
+  simp[namespaceTheory.nsLookup_def]>>
+  rw[]>>EVAL_TAC
+QED
+
+Theorem repl_types_ienv_ok:
+  ∀b (ffi:'ffi ffi_state) rs types s env.
+  repl_types b (ffi,rs) (types,s,env) ⇒
+  ienv_ok {} types
+Proof
+  Induct_on`repl_types`
+  \\ rw[infertype_prog_def, CaseEq"exc", init_infer_state_def]
+  \\ fs[PULL_EXISTS]
+  \\ qmatch_asmsub_abbrev_tac`infer_ds _ _ s0`
+  >- (
+    Cases_on`infer_ds init_config decs s0` \\ fs[] \\ rw[]
+    \\ drule (CONJUNCT2 infer_d_check)
+    \\ metis_tac[ienv_ok_extend_dec_ienv,ienv_ok_init_config])
+  >> (
+    Cases_on`infer_ds types decs s0` \\ fs[] \\ rw[]
+    \\ drule (CONJUNCT2 infer_d_check)
+    \\ metis_tac[ienv_ok_extend_dec_ienv,ienv_ok_init_config])
+QED
+
+Theorem convert_t_to_type:
+  convert_t(to_type t) = to_type_TS t
+Proof
+  Cases_on`t`>>EVAL_TAC
+QED
+
+Theorem check_ref_types_check_ref_types_TS:
+  check_ref_types ienv env x ⇒
+  check_ref_types_TS (ienv_to_tenv ienv) env x
+Proof
+  PairCases_on`x`>>
+  rw[check_ref_types_TS_def,check_ref_types_def]>>
+  fs[ienv_to_tenv_def,nsLookup_nsMap]>>
+  EVAL_TAC>>
+  fs[convert_t_to_type]
+QED
+
+Theorem repl_types_TS:
+  ∀(ffi:'ffi ffi_state) rs types s env.
+    repl_types F (ffi,rs) (types,s,env) ⇒
+    repl_types_TS (ffi,rs) (ienv_to_tenv types,s,env)
+Proof
+  Induct_on`repl_types`
+  \\ rw[infertype_prog_def, CaseEq"exc", init_infer_state_def]
+  \\ fs[PULL_EXISTS]
+  >- (
+    qmatch_asmsub_abbrev_tac`infer_ds _ _ s0`
+    \\ Cases_on`infer_ds init_config decs s0` \\ fs[] \\ rw[]
+    \\ drule (CONJUNCT2 infer_d_sound)
+    \\ disch_then (resolve_then Any mp_tac env_rel_init_config)
+    \\ impl_tac >- simp[Abbr`s0`] \\ strip_tac
+    \\ simp[ienv_to_tenv_extend,ienv_to_tenv_init_config]
+    \\ match_mp_tac repl_types_TS_init
+    \\ asm_exists_tac \\ simp[]
+    \\ qpat_x_assum`_ _ rs` mp_tac
+    \\ match_mp_tac EVERY_MONOTONIC
+    \\ rw[]
+    \\ simp[GSYM ienv_to_tenv_init_config, GSYM ienv_to_tenv_extend]
+    \\ match_mp_tac check_ref_types_check_ref_types_TS
+    \\ metis_tac[])
+  >- (
+    qmatch_asmsub_abbrev_tac`infer_ds _ _ s0`
+    \\ Cases_on`infer_ds types decs s0` \\ fs[] \\ rw[]
+    \\ drule (CONJUNCT2 infer_d_sound)
+    \\ disch_then(qspec_then `ienv_to_tenv types` mp_tac)
+    \\ impl_tac >- (
+      simp[Abbr`s0`]>>
+      metis_tac[repl_types_ienv_ok, env_rel_ienv_to_tenv])
+    \\ strip_tac
+    \\ simp[ienv_to_tenv_extend]
+    \\ metis_tac[repl_types_TS_eval])
+  >- (
+    qmatch_asmsub_abbrev_tac`infer_ds _ _ s0`
+    \\ Cases_on`infer_ds types decs s0` \\ fs[] \\ rw[]
+    \\ drule (CONJUNCT2 infer_d_sound)
+    \\ disch_then(qspec_then `ienv_to_tenv types` mp_tac)
+    \\ impl_tac >- (
+      simp[Abbr`s0`]>>
+      metis_tac[repl_types_ienv_ok, env_rel_ienv_to_tenv])
+    \\ strip_tac
+    \\ metis_tac[repl_types_TS_exn])
+  >- (
+    qmatch_asmsub_abbrev_tac`infer_ds _ _ s0`
+    \\ Cases_on`infer_ds types decs s0` \\ fs[] \\ rw[]
+    \\ drule (CONJUNCT2 infer_d_sound)
+    \\ disch_then(qspec_then `ienv_to_tenv types` mp_tac)
+    \\ impl_tac >- (
+      simp[Abbr`s0`]>>
+      metis_tac[repl_types_ienv_ok, env_rel_ienv_to_tenv])
+    \\ strip_tac
+    \\ metis_tac[repl_types_TS_exn_assign])
+  >>
+    metis_tac[repl_types_TS_str_assign]
+QED
+
+Definition ref_lookup_ok_def:
+  ref_lookup_ok refs (name:(string,string) id,ty,loc) =
+    ∃v:semanticPrimitives$v.
+      store_lookup loc refs = SOME (Refv v) ∧
+      (ty = Bool ⇒ v = Boolv T ∨ v = Boolv F) ∧
+      (ty = Str ⇒ ∃t. v = Litv (StrLit t))
+End
 
 Theorem repl_types_F_thm:
   ∀(ffi:'ffi ffi_state) rs types s env.
